\documentclass[a4paper,12pt]{article}
\usepackage{graphicx}
\usepackage[utf8]{inputenc}
\usepackage[russian]{babel}
\usepackage{amsmath,amssymb}
\usepackage{tikz}
\usepackage{pgfplots}
\pgfplotsset{compat=1.7}
\begin{document}

\begin{equation}
    \begin{array}{c}
    \sum_{i,j=0}^2 C_{ij}\frac{\partial U}{\partial j}\frac{\partial U}{\partial k}=
    \sum_{i,j=0}^2 C_{ij}\frac{(\sum_{m=0}^3\alpha_m\partial\phi_m)}
    {\partial j}\frac{(\sum_{m=0}^3\alpha_m\partial\phi_m)}{\partial k}= \\ \\
\end{array}
\end{equation} 

\begin{equation}
    \begin{array}{c}
        \frac{\partial}{\partial \alpha_{a}}:

        C_{00}
        (\frac{\partial\phi_{a}}{\partial 0}\frac{(\sum_{m=0}^3\alpha_m\partial\phi_m)}{\partial 0}+
        \frac{(\sum_{m=0}^3\alpha_m\partial\phi_m)}{\partial 0}\frac{\partial\phi_{a}}{\partial 0})+ \\ \\

        C_{01}
        (\frac{\partial\phi_{a}}{\partial 0}\frac{(\sum_{m=0}^3\alpha_m\partial\phi_m)}{\partial 1}+
        \frac{(\sum_{m=0}^3\alpha_m\partial\phi_m)}{\partial 0}\frac{\partial\phi_{a}}{\partial 1})+ \\ \\

        C_{10}
        (\frac{\partial\phi_{a}}{\partial 1}\frac{(\sum_{m=0}^3\alpha_m\partial\phi_m)}{\partial 0}+
        \frac{(\sum_{m=0}^3\alpha_m\partial\phi_m)}{\partial 1}\frac{\partial\phi_{a}}{\partial 0})+ \\ \\

        C_{11}
        (\frac{\partial\phi_{a}}{\partial 1}\frac{(\sum_{m=0}^3\alpha_m\partial\phi_m)}{\partial 1}+
        \frac{(\sum_{m=0}^3\alpha_m\partial\phi_m)}{\partial 1}\frac{\partial\phi_{a}}{\partial 1})\\ \\
\end{array}
\end{equation} 

\begin{equation}
    \begin{array}{c}
        \alpha_{b}*[

        C_{00}
        (\frac{\partial\phi_{a}}{\partial 0}\frac{\partial\phi_{b}}{\partial 0}+
        \frac{\partial\phi_{b}}{\partial 0}\frac{\partial\phi_{a}}{\partial 0})+ \\ \\

        C_{01}
        (\frac{\partial\phi_{a}}{\partial 0}\frac{\partial\phi_{b}}{\partial 1}+
        \frac{\partial\phi_{b}}{\partial 0}\frac{\partial\phi_{a}}{\partial 1})+ \\ \\

        C_{10}
        (\frac{\partial\phi_{a}}{\partial 1}\frac{\partial\phi_{b}}{\partial 0}+
        \frac{\partial\phi_{b}}{\partial 1}\frac{\partial\phi_{a}}{\partial 0})+ \\ \\

        C_{11}
        (\frac{\partial\phi_{a}}{\partial 1}\frac{\partial\phi_{b}}{\partial 1}+
        \frac{\partial\phi_{b}}{\partial 1}\frac{\partial\phi_{a}}{\partial 1}) ] = \\ \\
        \alpha_{b}*2*\sum_{i,j=0}^2C_{ij}\frac{\partial\phi_{a}}{\partial i}\frac{\partial\phi_{b}}{\partial j} \\ \\
\end{array}
\end{equation} 

\begin{equation}
    \begin{array}{c}
    \sum_{i,j,k,l=0}^2 C_{ijkl}\frac{\partial U_i}{\partial j}\frac{\partial U_l}{\partial k}=
    \sum_{i,j,k,l=0}^2 C_{ijkl}\frac{(\sum_{m=0}^3\alpha_m\partial\phi_m)_i}
    {\partial j}\frac{(\sum_{m=0}^3\alpha_m\partial\phi_m)_l}{\partial k}= \\ \\

    \sum_{j,k=0}^2 C_{0jk0}\frac{(\sum_{m=0}^3\alpha_m\partial\phi_m)_0}
    {\partial j}\frac{(\sum_{m=0}^3\alpha_m\partial\phi_m)_0}{\partial k}+ \\ \\

    \sum_{j,k=0}^2 C_{0jk1}\frac{(\sum_{m=0}^3\alpha_m\partial\phi_m)_0}
    {\partial j}\frac{(\sum_{m=0}^3\alpha_m\partial\phi_m)_1}{\partial k}+ \\ \\

    \sum_{j,k=0}^2 C_{0jk2}\frac{(\sum_{m=0}^3\alpha_m\partial\phi_m)_0}
    {\partial j}\frac{(\sum_{m=0}^3\alpha_m\partial\phi_m)_2}{\partial k}+ \\ \\


    \sum_{j,k=0}^2 C_{1jk0}\frac{(\sum_{m=0}^3\alpha_m\partial\phi_m)_1}
    {\partial j}\frac{(\sum_{m=0}^3\alpha_m\partial\phi_m)_0}{\partial k}+ \\ \\

    \sum_{j,k=0}^2 C_{1jk1}\frac{(\sum_{m=0}^3\alpha_m\partial\phi_m)_1}
    {\partial j}\frac{(\sum_{m=0}^3\alpha_m\partial\phi_m)_1}{\partial k}+ \\ \\

    \sum_{j,k=0}^2 C_{1jk2}\frac{(\sum_{m=0}^3\alpha_m\partial\phi_m)_1}
    {\partial j}\frac{(\sum_{m=0}^3\alpha_m\partial\phi_m)_2}{\partial k}+ \\ \\


    \sum_{j,k=0}^2 C_{2jk0}\frac{(\sum_{m=0}^3\alpha_m\partial\phi_m)_2}
    {\partial j}\frac{(\sum_{m=0}^3\alpha_m\partial\phi_m)_0}{\partial k}+ \\ \\

    \sum_{j,k=0}^2 C_{2jk1}\frac{(\sum_{m=0}^3\alpha_m\partial\phi_m)_2}
    {\partial j}\frac{(\sum_{m=0}^3\alpha_m\partial\phi_m)_1}{\partial k}+ \\ \\

    \sum_{j,k=0}^2 C_{2jk2}\frac{(\sum_{m=0}^3\alpha_m\partial\phi_m)_2}
    {\partial j}\frac{(\sum_{m=0}^3\alpha_m\partial\phi_m)_2}{\partial k} \\ \\
\end{array}
\end{equation} 

\begin{equation}
    \begin{array}{c}
        \frac{\partial}{\partial \alpha_{ab}}:

        \sum_{j,k=0}^2 C_{bjkb}\frac{\partial\phi_{ab}}{\partial j}
    \frac{(\sum_{m=0}^3\alpha_m\partial\phi_m)_b}{\partial k}+ \\ \\

    \sum_{j,k=0}^2 C_{bjkb}\frac{(\sum_{m=0}^3\alpha_m\partial\phi_m)_b}{\partial j}
    \frac{\partial\phi_{ab}}{\partial k}+ \\ \\

    \sum_{j,k=0}^2 C_{bjk\overline{b}}\frac{\partial\phi_{ab}}{\partial j}
    \frac{(\sum_{m=0}^3\alpha_m\partial\phi_m)_{\overline{b}}}{\partial k}+ \\ \\

    \sum_{j,k=0}^2 C_{bjk\overline{\overline{b}}}\frac{\partial\phi_{ab}}{\partial j}
    \frac{(\sum_{m=0}^3\alpha_m\partial\phi_m)_{\overline{\overline{b}}}}{\partial k}+ \\ \\

    \sum_{j,k=0}^2 C_{\overline{b}jkb}\frac{(\sum_{m=0}^3\alpha_m\partial\phi_m)_{\overline{b}}}{\partial j}
    \frac{\partial\phi_{ab}}{\partial k}+ \\ \\

    \sum_{j,k=0}^2 C_{\overline{\overline{b}}jkb}\frac{(\sum_{m=0}^3\alpha_m\partial\phi_m)_{\overline{\overline{b}}}}{\partial j}
    \frac{\partial\phi_{ab}}{\partial k}= \\ \\

    \sum_{j,k,l=0}^2 C_{ljkb}\frac{(\sum_{m=0}^3\alpha_m\partial\phi_m)_l}{\partial j}
    \frac{\partial\phi_{ab}}{\partial k}+ \\ \\

    \sum_{j,k,l=0}^2 C_{bjkl}\frac{\partial\phi_{ab}}{\partial j}
    \frac{(\sum_{m=0}^3\alpha_m\partial\phi_m)_l}{\partial k}= \\ \\

    2*\sum_{j,k,l=0}^2 C_{bjkl}\frac{\partial\phi_{ab}}{\partial j}
    \frac{(\sum_{m=0}^3\alpha_m\partial\phi_m)_l}{\partial k} \\ \\
\end{array}
\end{equation} 

\begin{equation}
    \begin{array}{c}
        \alpha_{cd}*
    2*\sum_{j,k=0}^2 C_{bjkd}\frac{\partial\phi_{ab}}{\partial j}
    \frac{\phi_{cd}}{\partial k} \\ \\
\end{array}
\end{equation} 
\end{document}













